update

Libs/maths.v
@@ -1,7 +1,7 @@
 Set Warnings "-notation-overridden".
 
 Require Import Coq.ZArith.ZArith.
-Require Import Coq.FSets.FMaps.
+Require Import Coq.Lists.List.
 Require Import Coq.Program.Program.
 
 Open Scope Z_scope.
@@ -136,10 +136,43 @@ Fixpoint expr_denote env (m : expr) : Z :=
   | Add x y => (expr_denote env x + expr_denote env y)%Z
   end.
 
+Fixpoint list_subst_expr  (l : list expr) (v v' : term) : list expr :=
+  match l with
+    | nil => nil
+    | h :: q => subst_expr h v v' :: list_subst_expr q v v'
+  end.
+
+Fixpoint subst_all_list_expr (x : list expr) (xs : list (term * term)) : list expr :=
+  match xs with
+  | nil => x
+  | cons (v, v') xs =>
+    subst_all_list_expr (list_subst_expr x v v') xs
+  end.
+
+Lemma subst_all_list_expr_nil defs : 
+  subst_all_list_expr nil defs = nil.
+Proof.
+  induction defs; simpl; intros; auto.
+  destruct a.
+  rewrite IHdefs; reflexivity.
+Qed.
+
+Lemma subst_all_list_expr_cons defs : forall x y,
+  subst_all_list_expr (x :: y) defs =
+  (subst_all_expr x defs) :: (subst_all_list_expr y defs).
+Proof.
+  induction defs; simpl; intros; auto.
+  destruct a.
+  rewrite IHdefs; reflexivity.
+Qed.
+
+Definition list_expr_denote env (l :list expr) : list Z := map (expr_denote env) l.
+
 Inductive formula :=
   | Top    : formula
   | Bottom : formula
   | Equal  : expr -> expr -> formula
+  | Equal_L : list expr -> list expr -> formula
   | Impl   : formula -> formula -> formula.
 
 Fixpoint subst_formula (t : formula) (v v' : term) : formula :=
@@ -147,6 +180,7 @@ Fixpoint subst_formula (t : formula) (v v' : term) : formula :=
   | Top => Top
   | Bottom => Bottom
   | Equal x y => Equal (subst_expr x v v') (subst_expr y v v')
+  | Equal_L x y => Equal_L (list_subst_expr x v v') (list_subst_expr y v v')
   | Impl p q => Impl (subst_formula p v v') (subst_formula q v v')
   end.
 
@@ -167,6 +201,15 @@ Qed.
 
 Lemma subst_all_formula_Bottom defs :
   subst_all_formula Bottom defs = Bottom.
+Proof.
+  induction defs; simpl; intros; auto.
+  destruct a.
+  rewrite IHdefs; reflexivity.
+Qed.
+
+Lemma subst_all_formula_Equal_L defs : forall x y,
+  subst_all_formula (Equal_L x y) defs =
+  Equal_L (subst_all_list_expr x defs) (subst_all_list_expr y defs).
 Proof.
   induction defs; simpl; intros; auto.
   destruct a.
@@ -196,6 +239,7 @@ Fixpoint formula_denote env (t : formula) : Prop :=
   | Top       => True
   | Bottom    => False
   | Equal x y => expr_denote env x = expr_denote env y
+  | Equal_L x y => list_expr_denote env x = list_expr_denote env y
   | Impl p q  => formula_denote env p -> formula_denote env q
   end.
 
@@ -210,11 +254,18 @@ Fixpoint expr_size (t : expr) : nat :=
   | Add x y => 1%nat + expr_size x + expr_size y
   end.
 
+Fixpoint list_expr_size (l: list expr) : nat :=
+  match l with 
+    |nil => 1%nat
+    | h :: q => 1%nat + expr_size h + list_expr_size q
+  end.
+
 Fixpoint formula_size (t : formula) : nat :=
   match t with
   | Top => 1%nat
   | Bottom => 1%nat
   | Equal x y => 1%nat + expr_size x + expr_size y
+  | Equal_L x y => 1%nat + list_expr_size x + list_expr_size y
   | Impl p q => formula_size p + formula_size q
   end.
 
@@ -230,6 +281,15 @@ Proof.
   - rewrite subst_all_expr_Add; simpl; auto.
 Qed.
 
+Lemma expr_size_subst_all_list_expr defs m :
+  list_expr_size (subst_all_list_expr m defs) = list_expr_size m.
+Proof.
+  induction m; simpl.
+  - rewrite subst_all_list_expr_nil; simpl; auto.
+  - rewrite subst_all_list_expr_cons; simpl;
+    rewrite expr_size_subst_all_expr; auto.
+Qed.
+
 Lemma formula_size_subst_all_formula defs q :
   formula_size (subst_all_formula q defs) = formula_size q.
 Proof.
@@ -238,6 +298,8 @@ Proof.
   - rewrite subst_all_formula_Bottom; simpl; auto.
   - rewrite subst_all_formula_Equal; simpl; auto.
     rewrite !expr_size_subst_all_expr; auto.
+  - rewrite subst_all_formula_Equal_L; simpl; auto.
+    repeat rewrite expr_size_subst_all_list_expr; auto.
   - rewrite subst_all_formula_Impl; simpl; auto.
 Qed.
 
@@ -313,6 +375,17 @@ Proof.
     rewrite IHt1, IHt2; auto.
 Qed.
 
+Lemma list_expr_substitution_eq env t xs :
+  Forall (fun p => term_denote env (fst p) = term_denote env (snd p)) xs
+    -> list_expr_denote env (subst_all_list_expr t (substitutions xs)) =
+       list_expr_denote env t.
+Proof.
+  induction t; simpl; intros.
+  - rewrite subst_all_list_expr_nil ; simpl ; auto.
+  - rewrite subst_all_list_expr_cons ; simpl.
+    rewrite expr_substitution_eq, IHt; auto.
+Qed.
+
 Lemma formula_substitution_eq env t xs :
   Forall (fun p => term_denote env (fst p) = term_denote env (snd p)) xs
     -> formula_denote env (subst_all_formula t (substitutions xs)) =
@@ -323,6 +396,8 @@ Proof.
   - rewrite subst_all_formula_Bottom; simpl; auto.
   - rewrite subst_all_formula_Equal; simpl; intros.
     rewrite !expr_substitution_eq; auto.
+  - rewrite subst_all_formula_Equal_L; simpl; intros.
+    rewrite !list_expr_substitution_eq; auto.
   - rewrite subst_all_formula_Impl; simpl; intros.
     intuition.
     rewrite H0, H1; auto.
@@ -332,22 +407,47 @@ Qed.
  * Computational decision procedure for map membership
  *)
 
+Definition decision (env : environment) (m n : expr) : bool :=
+  Z.eqb (expr_denote env m) (expr_denote env n).
+
+Lemma decision_eq : forall env x y, decision env x y = true -> expr_denote env x = expr_denote env y.
+Proof. intros ; unfold decision in H ; apply Z.eqb_eq in H ; auto. Qed.
+
+Fixpoint list_decision (env : environment) (m n : list expr) : bool :=
+  match m,n with
+    | nil,nil => true
+    | h1::q1, h2::q2 => decision env h1 h2 && list_decision env q1 q2
+    | _ , _ => false
+  end.
+
+Lemma list_decision_eq : forall env n m, list_decision env m n = true -> 
+  list_expr_denote env m = list_expr_denote env n.
+Proof.
+  induction n ; intros [] Heq ; simpl in * ; try congruence.
+  apply Bool.andb_true_iff in Heq ; destruct Heq as [Hdec Hlistdec].
+  f_equal.
+  apply decision_eq ; assumption.
+  auto.
+Qed.
+
+
 Program Definition formula_forward (t : formula) env (hyp : formula)
         (cont : forall env' defs, [formula_denote env' (subst_all_formula t defs)]) :
   [formula_denote env hyp -> formula_denote env t] :=
   match hyp with
   | Top => Reduce (cont env nil)
   | Bottom => Yes
-  | Equal x y => No             (* Benoit: TODO *)
+(*   | Equal x y => match x,y with 
+                  | Ref a,Ref b => Reduce (cont env [(a,b)])
+                  | _, _ => Reduce (cont env nil)
+ *)
+  | Equal x y => No (* TODO *)
+  | Equal_L x y => No (* TODO *)
   | Impl _ _ => Reduce (cont env nil)
   end.
 Next Obligation.
   contradiction.
 Defined.
-
-(* Benoit: TODO: This should be changed to fit your problem. *)
-Definition decision (env : environment) (m n : expr) : bool :=
-  Z.eqb (expr_denote env m) (expr_denote env n).
 
 Program Fixpoint formula_backward (t : formula) env {measure (formula_size t)} :
   [formula_denote env t] :=
@@ -358,15 +458,19 @@ Program Fixpoint formula_backward (t : formula) env {measure (formula_size t)} :
                  | true => Yes
                  | false => No
                  end
+  | Equal_L x y => match list_decision env x y with
+                 | true => Yes
+                 | false => No
+                 end
   | Impl p q =>
     formula_forward q env p
       (fun env' defs' => formula_backward (subst_all_formula q defs') env')
   end.
 Next Obligation.
-  unfold decision in Heq_anonymous.
-  symmetry in Heq_anonymous.
-  apply Z.eqb_eq in Heq_anonymous.
-  assumption.
+  apply decision_eq ; auto.
+Defined.
+Next Obligation.
+  apply list_decision_eq ; auto.
 Defined.
 Next Obligation.
   rewrite formula_size_subst_all_formula; simpl.
@@ -437,13 +541,19 @@ Ltac allVars xs e :=
   | ?X + ?Y =>
     let xs := allVar xs X in
     allVar xs Y
+  | nil = nil => xs
+  | ?hp :: ?qp = ?hq :: ?qq => 
+    let xs1 := allVars xs hp in
+    let xs2 := allVars xs1 qp in
+    let xs3 := allVars xs2 hq in
+    allVars xs3 qq
   | ?P = ?Q =>
     let xs := allVars xs P in
     allVars xs Q
   | ?P -> ?Q =>
     let xs := allVars xs P in
     allVars xs Q
-  | ?X => allVar xs X           (* Benoit: TODO: This may be too open *)
+(*  | ?X => allVar xs X           (* Benoit: TODO: This may be too open *)*)
   | _ => xs
   end.
 
@@ -473,6 +583,11 @@ Ltac reifyExpr env t :=
     let x := reifyExpr env X in
     let y := reifyExpr env Y in
     constr:(Add x y)
+  | nil => constr:(nil)
+  | ?X :: ?Y =>
+    let x := reifyExpr env X in
+    let y := reifyExpr env Y in
+    constr:(cons x y)
   | ?X =>
     let x := reifyValue env X in
     constr:(Ref x)
@@ -524,7 +639,11 @@ Ltac reify :=
  *)
 
 Ltac maths := reify; apply formula_sound; vm_compute; auto.
-
-Goal 2 * 3 = 3 * 2.
-  maths.
-Qed.
+(*
+Goal forall x, (2*3*4*x = 3*4*2*x)%Z.
+  intros.
+  reify.
+  apply formula_sound.
+  vm_compute.
+  
+Qed.*)
