Op/M.v
@@ -7,18 +7,6 @@ Require Import stdpp.prelude.
 
 Local Open Scope Z.
 
-Lemma ZscalarMult_bound_const: forall (m2 n2 o p a: Z) (b: list Z),
-  0 <= a ->
-  Forall (fun x => m2 <= x <= n2) b -> 
-  o = a * m2 ->
-  p = a * n2 ->
-  Forall (fun x => o <= x <= p) (a ∘∘ b).
-Proof.
-  introv Ha Hb Ho Hp.
-  rewrite ZscalarMult_eq_ZunopList.
-  eapply (Forall_ZunopList _ (fun x : ℤ => a = x) (fun x : ℤ => m2 <= x <= n2)) ; go.
-Qed.
-
 Lemma ZscalarMult_bound_inter: forall (m1 n1 m2 n2 o p a: Z) (b: list Z),
   (fun x => m1 <= x <= n1) a ->
   Forall (fun x => m2 <= x <= n2) b -> 
